Implementation of "bare zero" numerals.

src/num/Num_conv.sml
@@ -14,7 +14,7 @@
 structure Num_conv :> Num_conv =
 struct
 
-open HolKernel basicHol90Lib Parse;
+open HolKernel basicHol90Lib Parse Psyntax;
 
 (* this code no longer needs to use mk_thm, because numbers are no
    longer an infinite family of constants but rather built-up in a
@@ -25,44 +25,30 @@ fun NUM_CONV_ERR function message =
                  origin_function = function,
                  message = message}
 
-fun mk_comb(t1, t2) = Term.mk_comb{Rand = t2, Rator = t1}
 val N = ==`:num`==
-val ZERO = --`ZERO`--
+val ZERO = --`0`--
 val SUC = --`SUC`--
 val PRE = --`PRE`--
 val bit1 = --`NUMERAL_BIT1`--
 val bit2 = --`NUMERAL_BIT2`--
-val numeral = --`NUMERAL`--
-val numzero = mk_comb(numeral, ZERO)
 val eq = --`$= :num->num->bool`--
 val lt_0 = --`$< 0`--
 
-fun is_numeral t = let
-  fun is_n t =
-    if (is_const t) then
-      if (t = ZERO) then true
-      else false
-    else if (is_comb t) then let
-      val {Rator, Rand} = dest_comb t
-    in
-      ((Rator = bit1) orelse (Rator = bit2)) andalso is_n Rand
-    end
-    else false
-in
-  is_comb t andalso #Rator(dest_comb t) = numeral andalso
-  is_n (#Rand(dest_comb t))
-end
-
 val PRE_SUC_EQ = arithmeticTheory.PRE_SUC_EQ
   (* |- !m n. 0 < n ==> ((m = PRE n) = SUC m = n) *)
+val save_zero = prove(Term`NUMERAL ALT_ZERO = 0`,
+                      REWRITE_TAC [arithmeticTheory.NUMERAL_DEF,
+                                   arithmeticTheory.ALT_ZERO]);
+
 val numeral_pre = numeralTheory.numeral_pre
 val numeral_lt = numeralTheory.numeral_lt
 val numeral_distrib = numeralTheory.numeral_distrib
 
 fun num_CONV t =
-  if is_numeral t andalso t <> numzero then let
+  if is_numeral t andalso t <> ZERO then let
     val pre_t = mk_comb(PRE, t)
-    val pre_thm = SYM (REWRITE_CONV [numeral_pre, numeral_distrib] pre_t)
+    val pre_thm =
+      SYM (REWRITE_CONV [numeral_pre, numeral_distrib, save_zero] pre_t)
     val result_t = lhs (concl pre_thm)
     val lt_t = mk_comb(lt_0, t)
     val less_thm = EQT_ELIM (REWRITE_CONV [numeral_lt, numeral_distrib] lt_t)
