src/parse/Parse_support.sml
@@ -5,7 +5,7 @@ type hol_type = Type.hol_type;
 
 open Exception Lib;
 
-fun PARSE_SUPPORT_ERR function message = 
+fun PARSE_SUPPORT_ERR function message =
  Exception.HOL_ERR{origin_structure = "Parse_support",
                    origin_function = function,
                    message = message};
@@ -19,7 +19,7 @@ datatype arg = Rec_occ | Hty of hol_type;
  * The three kinds of objects parsable by the hol.yak file: preterms, types,
  * and datatype declarations.
  *---------------------------------------------------------------------------*)
-datatype parse = 
+datatype parse =
      PTM of Preterm.preterm
    | TY of hol_type
    | TY_SPEC of {ty_name: string,
@@ -27,7 +27,7 @@ datatype parse =
 
 
 
-type env = {scope : (string * hol_type) list, 
+type env = {scope : (string * hol_type) list,
             free  : (string * hol_type) list};
 
 fun lookup_fvar(s,({free,...}:env)) = assoc s free;
@@ -46,8 +46,8 @@ type preterm_in_env = env -> Preterm.preterm * env
 type bvar_in_env = env -> (Preterm.preterm -> Preterm.preterm) * env
 
 (*---------------------------------------------------------------------------
- * Denotes a variable bound by a binder ("\\" or a constant, e.g., 
- * "!", "?", "@"). Hence, it takes a binder and returns a function from 
+ * Denotes a variable bound by a binder ("\\" or a constant, e.g.,
+ * "!", "?", "@"). Hence, it takes a binder and returns a function from
  * the body to a preterm (plus of course, any changes to the env).
  *---------------------------------------------------------------------------*)
 type binder_in_env = string -> bvar_in_env
@@ -55,13 +55,13 @@ type binder_in_env = string -> bvar_in_env
 
 
 (*---------------------------------------------------------------------------
- * Top level parse terms 
+ * Top level parse terms
  *---------------------------------------------------------------------------*)
 fun make_preterm tm_in_e = fst(tm_in_e empty_env)
 
 
 (*---------------------------------------------------------------------------
- * Antiquotes 
+ * Antiquotes
  *---------------------------------------------------------------------------*)
 fun make_aq tm E = (Preterm.Antiq tm, E)
 
@@ -74,9 +74,9 @@ local val ren_ref = ref (fn _:(int,hol_type)Lib.istream =>
       val _ = Type.Ps_init ren_ref
       val rename_tv = !ren_ref
 in
-fun gen_const tyvars s = 
+fun gen_const tyvars s =
    let val {Name,Ty} = Term.dest_const(#const(Term.const_decl s))
-   in Preterm.Const 
+   in Preterm.Const
         (case (rename_tv tyvars Ty)
            of Type.SAME     => {Name=Name, Ty=Ty}
             | Type.DIFF ty' => {Name=Name, Ty=ty'})
@@ -88,9 +88,9 @@ end;
 (*---------------------------------------------------------------------------
  * Binding occurrences of variables
  *---------------------------------------------------------------------------*)
-fun make_binding_occ tyvars s "\\" E = 
+fun make_binding_occ tyvars s "\\" E =
      let val ntv = Lib.state(Lib.next tyvars)
-     in ((fn b => Preterm.Abs{Bvar = Preterm.Var{Name = s, Ty = ntv}, 
+     in ((fn b => Preterm.Abs{Bvar = Preterm.Var{Name = s, Ty = ntv},
                               Body = b}),
          add_scope((s,ntv),E))
      end
@@ -102,9 +102,9 @@ fun make_binding_occ tyvars s "\\" E =
          add_scope((s,ntv),E))
      end;
 
-fun make_aq_binding_occ _ aq "\\" E = 
+fun make_aq_binding_occ _ aq "\\" E =
      ((fn b => Preterm.Abs{Bvar=Preterm.Antiq aq,Body=b}), E)
-  | make_aq_binding_occ tyvars aq binder E = 
+  | make_aq_binding_occ tyvars aq binder E =
         ((fn b => Preterm.Comb{Rator = gen_const tyvars binder,
                                Rand = Preterm.Abs{Bvar = Preterm.Antiq aq,
                                                   Body = b}}),  E);
@@ -138,12 +138,13 @@ fun int2numeral tyvars nstr =
 fun make_num_literal tyvars (s,E) =
   if Globals.nums_defined()
   then (int2numeral tyvars s, E)
-  else make_free_var tyvars (s,E);
+  else raise PARSE_SUPPORT_ERR "make_num_literal"
+    "numbers not yet defined - load \"arithmeticTheory\""
 
 (*---------------------------------------------------------------------------
  * Makes the assumption that s is already quoted (except for emptystring).
  *---------------------------------------------------------------------------*)
-fun make_string s E = 
+fun make_string s E =
    let val atom = {Name=s, Ty=Type.mk_type{Tyop="string",Args=[]}}
        val tag = if Globals.strings_defined()
                  then Preterm.Const else Preterm.Var
@@ -153,7 +154,7 @@ fun make_string s E =
 
 (* Atoms *)
 local val the_hidden = ref [] : string list ref
-in 
+in
  fun hidden s = mem s (!the_hidden)
  fun hide s = (the_hidden := insert s (!the_hidden))
  fun reveal s = (the_hidden := set_diff (!the_hidden) [s])
@@ -163,10 +164,10 @@ end;
  * Identifiers work as follows: look for the string in the scope;
  * if it's there, put the var. Otherwise, the string might be a constant that
  * we intend to parse as a free var. Otherwise, the string might be a constant;
- * look in the symbol table. If it's there, rename any type variables in 
+ * look in the symbol table. If it's there, rename any type variables in
  * its binding and make a Const out of it. Otherwise, it's not in the scope
  * and not in the symtab, hence is a free variable. Generate a new type
- * variable and bind the term variable to it in E; also we return a var 
+ * variable and bind the term variable to it in E; also we return a var
  * that has the new type variable as its type.
  *
  * Free vars are placed in the "free" part of the environment; this is a
@@ -174,7 +175,7 @@ end;
  * of an Abs, we return the scope in effect when entering the Abs, but the
  * "free"s include new ones found in the body of the Abs.
  *
- * Note: this code should maybe check whether the prospective identifier is a 
+ * Note: this code should maybe check whether the prospective identifier is a
  * reserved word  or not.
  *---------------------------------------------------------------------------*)
 fun make_atom tyvars s E =
@@ -183,22 +184,22 @@ fun make_atom tyvars s E =
    => if (hidden s)
       then make_free_var tyvars (s,E)
       else (gen_const tyvars s, E)
-           handle HOL_ERR _ 
+           handle HOL_ERR _
              => if (Lexis.is_num_literal s)
                 then make_num_literal tyvars (s,E)
                 else make_free_var tyvars (s,E);
 
 
 (*---------------------------------------------------------------------------
- * Combs 
+ * Combs
  *---------------------------------------------------------------------------*)
 fun list_make_comb (tm1::(rst as (_::_))) E =
-   rev_itlist (fn tm => fn (trm,e) => 
+   rev_itlist (fn tm => fn (trm,e) =>
       let val (tm',e') = tm e
       in (Preterm.Comb{Rator = trm, Rand = tm'}, e') end)     rst (tm1 E) ;
 
 (*---------------------------------------------------------------------------
- * Constraints 
+ * Constraints
  *---------------------------------------------------------------------------*)
 fun make_constrained tm ty E =
    let val (tm',E') = tm E
@@ -208,10 +209,10 @@ fun make_constrained tm ty E =
 
 (*---------------------------------------------------------------------------
  * Abstractions, qualified abstractions, and vstructs.
- * The thing to know about parsing abstractions is that an abstraction is 
- * a function from the string identifying the binder to an env to a 
+ * The thing to know about parsing abstractions is that an abstraction is
+ * a function from the string identifying the binder to an env to a
  * pair. The first member of the pair is a function that will take the body
- * of the abstraction and produce a lambda term, essentially by clapping 
+ * of the abstraction and produce a lambda term, essentially by clapping
  * on whatever variables, or applying whatever constants necessary. The second
  * member of the pair is the environment previous to entering the abstraction
  * plus whatever new free variables were found in the body of the abstraction.
@@ -221,23 +222,23 @@ fun make_constrained tm ty E =
  *---------------------------------------------------------------------------*)
 
 fun bind_term binder alist tm (E as {scope=scope0,...}:env) =
-   let val (E',F) = rev_itlist (fn a => fn (e,f) => 
+   let val (E',F) = rev_itlist (fn a => fn (e,f) =>
              let val (g,e') = a binder e in (e', f o g) end) alist (E,I)
        val (tm',({free=free1,...}:env)) = tm E'
    in (F tm', {scope=scope0,free=free1})
    end;
 
-fun restr_binder s = 
+fun restr_binder s =
    assoc s (Dsyntax.binder_restrictions()) handle HOL_ERR _
    => raise PARSE_SUPPORT_ERR "restr_binder"
                       ("no restriction associated with "^Lib.quote s)
 
 fun bind_restr_term tyvars binder vlist restr tm (E as {scope=scope0,...}:env)=
-   let fun replicate_rbinder e = 
+   let fun replicate_rbinder e =
             (gen_const tyvars (restr_binder binder),e)
              handle HOL_ERR _ => raise PARSE_SUPPORT_ERR "bind_restr_term"
               ("Can't find constant associated with "^Lib.quote binder)
-       val (E',F) = 
+       val (E',F) =
           rev_itlist (fn v => fn (e,f)
              => let val (prefix,e') = list_make_comb[replicate_rbinder,restr] e
                     val (g,e'') = v "\\" e'
@@ -250,57 +251,57 @@ fun bind_restr_term tyvars binder vlist restr tm (E as {scope=scope0,...}:env)=
 
 
 fun split ty =
-  case (Type.dest_type ty) 
+  case (Type.dest_type ty)
    of {Tyop="prod",Args} => Args
     | _ => raise PARSE_SUPPORT_ERR "split" "not a product";
 
 
 
 fun cdom M [] = M
-  | cdom (Preterm.Abs{Bvar,Body}) (ty::rst) = 
-       Preterm.Abs{Bvar = Preterm.Constrained(Bvar,ty), 
+  | cdom (Preterm.Abs{Bvar,Body}) (ty::rst) =
+       Preterm.Abs{Bvar = Preterm.Constrained(Bvar,ty),
                    Body = cdom Body rst}
-  | cdom (Preterm.Comb{Rator as Preterm.Const{Name="UNCURRY",...},Rand}) 
-         (ty::rst) = 
-       Preterm.Comb{Rator=Rator, Rand=cdom Rand (split ty@rst)} 
+  | cdom (Preterm.Comb{Rator as Preterm.Const{Name="UNCURRY",...},Rand})
+         (ty::rst) =
+       Preterm.Comb{Rator=Rator, Rand=cdom Rand (split ty@rst)}
   | cdom x y = raise PARSE_SUPPORT_ERR"cdom" "missing case"
 
 
 fun cdomf (f,e) ty = ((fn tm => cdom (f tm) [ty]), e)
 
-fun make_vstruct tyvars bvl tyo binder E = 
+fun make_vstruct tyvars bvl tyo binder E =
  let fun loop ([v],E) = v "\\" E
-       | loop ((v::rst),E) = 
+       | loop ((v::rst),E) =
            let val (f,e) = v "\\" E
                val (F,E') = loop(rst,e)
            in ((fn b => Preterm.Comb{Rator = gen_const tyvars "UNCURRY",
                                      Rand = f(F b)}), E') end
        | loop _ = raise PARSE_SUPPORT_ERR"make_vstruct"
                                          "impl. error, empty vstruct"
-     val (F,E') = case tyo 
-                  of NONE    => loop(bvl,E) 
+     val (F,E') = case tyo
+                  of NONE    => loop(bvl,E)
                    | SOME ty => cdomf (hd bvl "\\" E) ty
    in
-   case binder 
+   case binder
    of "\\" => (F,E')
     | _ => ((fn b => Preterm.Comb{Rator=gen_const tyvars binder,Rand=F b}), E')
    end;
 
 
 (*---------------------------------------------------------------------------
- * Let bindings 
+ * Let bindings
  *---------------------------------------------------------------------------*)
 fun make_let tyvars bindings tm env =
    let val {body_bvars, args, E} =
           itlist (fn (bvs,arg) => fn {body_bvars,args,E} =>
                     let val (b::rst) = bvs
-                        val (arg',E') = 
+                        val (arg',E') =
                           case rst of [] => arg E | L => bind_term "\\" L arg E
                     in {body_bvars = b::body_bvars, args = arg'::args, E = E'}
                     end) bindings {body_bvars = [], args = [], E = env}
        val (core,E') = bind_term "\\" body_bvars tm E
    in
-   ( rev_itlist (fn arg => fn core => 
+   ( rev_itlist (fn arg => fn core =>
        Preterm.Comb{Rator=Preterm.Comb{Rator=gen_const tyvars"LET",Rand=core},
                     Rand = arg}) args core,
      E')  end
@@ -313,25 +314,25 @@ fun make_let tyvars bindings tm env =
  * This is a bit tricky in the case that alist = [], for we still do a
  * make_atom "CONS". But we know that "CONS" is already in the symtab, hence
  * make_atom "CONS" E = (Const{Name = "CONS", Ty = ...},E') and E = E'.
- * So nothing new can get added to the environment. When it builds the 
+ * So nothing new can get added to the environment. When it builds the
  * environment, it goes right-to-left in the list, so maybe error messages
  * will be puzzling.
  *---------------------------------------------------------------------------*)
 fun make_list tyvars alist E =
- let val (cons,E') = make_atom tyvars "CONS" E   
+ let val (cons,E') = make_atom tyvars "CONS" E
  in itlist (fn h => fn (L,E) =>
      let val (h',E') = h E
      in (Preterm.Comb{Rator=Preterm.Comb{Rator=cons,Rand=h'}, Rand=L}, E') end)
    alist (make_atom tyvars "NIL" E')
  end;
 
-fun make_set_const tyvars fname s E = 
+fun make_set_const tyvars fname s E =
  (gen_const tyvars s, E) handle HOL_ERR _
-  => raise PARSE_SUPPORT_ERR fname 
+  => raise PARSE_SUPPORT_ERR fname
        ("The theory "^Lib.quote "set"^" is not loaded");
 
 (*---------------------------------------------------------------------------
- * You can't make a set unless the theory of sets is an ancestor. 
+ * You can't make a set unless the theory of sets is an ancestor.
  *  The calls to make_set_const ensure this.
  *---------------------------------------------------------------------------*)
 fun make_set tyvars [] E = make_set_const tyvars "make_set" "EMPTY" E
@@ -346,14 +347,14 @@ fun make_set tyvars [] E = make_set_const tyvars "make_set" "EMPTY" E
 
 
 (*---------------------------------------------------------------------------
- * Set abstractions {tm1 | tm2}. The complicated rigamarole at the front is 
- * so that new type variables only get made once per free var, although we 
+ * Set abstractions {tm1 | tm2}. The complicated rigamarole at the front is
+ * so that new type variables only get made once per free var, although we
  * compute the free vars for tm1 and tm2 separately.
  *
  * Warning: apt not to work if you want to "antiquote in" free variables that
  * will subsequently get bound in the set abstraction.
  *---------------------------------------------------------------------------*)
-fun make_set_abs tyvars (tm1,tm2) (E as {scope=scope0,...}:env) = 
+fun make_set_abs tyvars (tm1,tm2) (E as {scope=scope0,...}:env) =
    let val (_,(e1:env)) = tm1 empty_env
        val (_,(e2:env)) = tm2 empty_env
        val (_,(e3:env)) = tm2 e1
@@ -365,10 +366,10 @@ fun make_set_abs tyvars (tm1,tm2) (E as {scope=scope0,...}:env) =
    case (gather (fn (name,_) => mem name fv_names) init_fv)
      of [] => raise PARSE_SUPPORT_ERR"make_set_abs"
                                 "no free variables in set abstraction"
-      | quants => 
-         let val quants' = map 
+      | quants =>
+         let val quants' = map
                 (fn (bnd as (Name,Ty)) =>
-                     (fn (s:string) => fn E => 
+                     (fn (s:string) => fn E =>
                        ((fn b => Preterm.Abs{Bvar=Preterm.Var{Name=Name,Ty=Ty},
                                              Body=b}),
                                 add_scope(bnd,E))))
@@ -387,7 +388,7 @@ fun make_set_abs tyvars (tm1,tm2) (E as {scope=scope0,...}:env) =
 val rec_occ = Type.dummy
 
 fun make_atomic_type (ident,NONE) = Type.mk_type{Tyop=ident, Args=[]}
-  | make_atomic_type (ident,SOME s) = 
+  | make_atomic_type (ident,SOME s) =
      if (ident = s) then rec_occ
      else make_atomic_type(ident,NONE);
 
@@ -397,9 +398,9 @@ fun make_type_app (s,tylist) = Type.mk_type{Tyop=s, Args=tylist}
 (*---------------------------------------------------------------------------
  * Clauses in type specifications
  *
- * Recursive occurrences of the defined type are marked with Type.dummy, a 
- * nonsense type variable, in order to stay within the the type of 
- * hol_types (this saves on creating a new type built from Rec_occs and 
+ * Recursive occurrences of the defined type are marked with Type.dummy, a
+ * nonsense type variable, in order to stay within the the type of
+ * hol_types (this saves on creating a new type built from Rec_occs and
  * normal hol_types).
  *---------------------------------------------------------------------------*)
 fun make_type_clause {constructor, args} =
@@ -413,13 +414,13 @@ fun make_type_clause {constructor, args} =
                   of {Args=[],Tyop}   => ()
                    | {Args,Tyop} => (map check Args; ())
 
-     fun munge ty = 
-       if (ty = rec_occ) then Rec_occ else 
+     fun munge ty =
+       if (ty = rec_occ) then Rec_occ else
        if (Type.is_vartype ty) then Hty ty
        else case Type.dest_type ty
             of {Args=[],Tyop} => Hty ty
              | {Args,Tyop}    => (map check Args; Hty ty)
- in 
+ in
     {constructor=constructor, args = map munge args}
  end;
 
@@ -449,7 +450,7 @@ fun list_make_list tmlist E =
    end;
 
 fun G [] (f,arg) = [(f,arg)]
-  | G (stk as ((g,tm)::stk')) (f,arg) = 
+  | G (stk as ((g,tm)::stk')) (f,arg) =
         if (prec g >= prec f)
         then let val tm' = Preterm.Comb{Rator = Preterm.Comb{Rator=g,Rand=arg},
                                         Rand = tm}
